vput

steel/apps/kvstore/Zeta.Steel.Application.fst
@@ -63,6 +63,13 @@ let vget_app_success (tsm:TSM.thread_state_model) (r:F.vget_args_t)
     let r, _, _ = S.vget_spec_f (vget_spec_args r) recs in
     App.Fn_success? r
 
+let vget_impl_tsm
+  (tsm:TSM.thread_state_model)
+  (r:F.vget_args_t)
+  (store_kv:(F.key_t & option F.value_t){slot_value_is_kv tsm r.vget_slot store_kv})
+  : TSM.thread_state_model
+  = tsm
+
 let vget_impl (#tsm:TSM.thread_state_model)
   (t:VT.thread_state_t)
   (r:F.vget_args_t)
@@ -71,7 +78,7 @@ let vget_impl (#tsm:TSM.thread_state_model)
       (VT.thread_state_inv_core t tsm)
       (fun b -> 
        if b
-       then VT.thread_state_inv_core t tsm
+       then VT.thread_state_inv_core t (vget_impl_tsm tsm r store_kv)
        else VT.thread_state_inv_core t tsm)
       (requires True)
       (ensures fun b ->
@@ -82,9 +89,9 @@ let vget_impl (#tsm:TSM.thread_state_model)
     then if Some r.vget_value = snd store_kv
          then begin
            let b = true in
-           rewrite (VT.thread_state_inv_core t tsm)
+           rewrite (VT.thread_state_inv_core t (vget_impl_tsm tsm r store_kv))
                    (if b
-                    then VT.thread_state_inv_core t tsm
+                    then VT.thread_state_inv_core t (vget_impl_tsm tsm r store_kv)
                     else VT.thread_state_inv_core t tsm);
            return b           
          end
@@ -92,7 +99,7 @@ let vget_impl (#tsm:TSM.thread_state_model)
            let b = false in
            rewrite (VT.thread_state_inv_core t tsm)
                    (if b
-                    then VT.thread_state_inv_core t tsm
+                    then VT.thread_state_inv_core t (vget_impl_tsm tsm r store_kv)
                     else VT.thread_state_inv_core t tsm);
            return b
          end
@@ -100,7 +107,7 @@ let vget_impl (#tsm:TSM.thread_state_model)
       let b = false in
       rewrite (VT.thread_state_inv_core t tsm)
               (if b
-               then VT.thread_state_inv_core t tsm
+               then VT.thread_state_inv_core t (vget_impl_tsm tsm r store_kv)
                else VT.thread_state_inv_core t tsm);
       return b
     end
@@ -152,22 +159,15 @@ let run_vget
             let b = vget_impl t r (k, vopt) in
             if b
             then begin
-              let tsm_impl = tsm in
               rewrite (if b
-                       then VT.thread_state_inv_core t tsm
+                       then VT.thread_state_inv_core t (vget_impl_tsm tsm r (k, vopt))
                        else VT.thread_state_inv_core t tsm)
-                      (if b
-                       then VT.thread_state_inv_core t tsm_impl
-                       else VT.thread_state_inv_core t tsm);
-              rewrite (if b
-                       then VT.thread_state_inv_core t tsm_impl
-                       else VT.thread_state_inv_core t tsm)
-                      (VT.thread_state_inv_core t tsm_impl);
+                      (VT.thread_state_inv_core t (vget_impl_tsm tsm r (k, vopt)));
               let tsm_write_slots =
                 TSM.write_slots tsm (vget_spec_slots r)
                                     (vget_spec_out_vals tsm r) in
-              assert (Seq.equal tsm_impl.store tsm_write_slots.store);
-              rewrite (VT.thread_state_inv_core t tsm_impl)
+              assert (Seq.equal (vget_impl_tsm tsm r (k, vopt)).store tsm_write_slots.store);
+              rewrite (VT.thread_state_inv_core t (vget_impl_tsm tsm r (k, vopt)))
                       (VT.thread_state_inv_core t tsm_write_slots);
 
               assume (Zeta.SeqAux.distinct_elems_comp (vget_spec_slots r));
@@ -198,7 +198,187 @@ let run_vget
             end
             else begin
               rewrite (if b
-                       then VT.thread_state_inv_core t tsm
+                       then VT.thread_state_inv_core t (vget_impl_tsm tsm r (k, vopt))
+                       else VT.thread_state_inv_core t tsm)
+                      (VT.thread_state_inv_core t tsm);
+              VT.intro_thread_state_inv t;
+              return Run_app_verify_failure
+            end
+        end
+        else return Run_app_verify_failure
+      end
+      else return Run_app_parsing_failure
+#pop-options
+
+let vput_spec_args (r:F.vput_args_t)
+  : GTot (App.interp_code S.adm S.vput_spec_arg_t)
+  = r.vput_key, r.vput_value
+
+let vput_spec_slots (r:F.vput_args_t)
+  : GTot (Seq.seq slot_id)
+  = Seq.create 1 r.vput_slot
+
+let vput_spec_out_vals (tsm:TSM.thread_state_model) (r:F.vput_args_t)
+  : Ghost (r:Seq.seq (App.app_value_nullable S.adm){Seq.length r == S.vput_spec_arity})
+          (requires Some? (TSM.read_slots tsm (vput_spec_slots r)))
+          (ensures fun _ -> True)
+  = let recs = Some?.v (TSM.read_slots tsm (vput_spec_slots r)) in
+    let _, _, out_vals = S.vput_spec_f (vput_spec_args r) recs in
+    out_vals
+
+let vput_app_result (tsm:TSM.thread_state_model) (r:F.vput_args_t)
+  : Ghost app_result_entry
+      (requires Some? (TSM.read_slots tsm (vput_spec_slots r)))
+      (ensures fun _ -> True)
+  = let recs = Some?.v (TSM.read_slots tsm (vput_spec_slots r)) in
+    let _, res, _ = S.vput_spec_f (vput_spec_args r) recs in  
+    (| S.vput_id, vput_spec_args r, recs, res |)
+
+let vput_app_success (tsm:TSM.thread_state_model) (r:F.vput_args_t)
+  : Ghost bool
+      (requires Some? (TSM.read_slots tsm (vput_spec_slots r)))
+      (ensures fun _ -> True)
+  = let recs = Some?.v (TSM.read_slots tsm (vput_spec_slots r)) in
+    let r, _, _ = S.vput_spec_f (vput_spec_args r) recs in
+    App.Fn_success? r
+
+let vput_impl_tsm
+  (tsm:TSM.thread_state_model)
+  (r:F.vput_args_t)
+  (store_kv:(F.key_t & option F.value_t){slot_value_is_kv tsm r.vput_slot store_kv})
+  : TSM.thread_state_model
+  = VT.update_tsm_slot_value tsm r.vput_slot (DValue (Some r.vput_value))
+
+let vput_impl (#tsm:TSM.thread_state_model)
+  (t:VT.thread_state_t)
+  (r:F.vput_args_t)
+  (store_kv:(F.key_t & option F.value_t){slot_value_is_kv tsm r.vput_slot store_kv})
+  : ST bool
+      (VT.thread_state_inv_core t tsm)
+      (fun b -> 
+       if b
+       then VT.thread_state_inv_core t (vput_impl_tsm tsm r store_kv)
+       else VT.thread_state_inv_core t tsm)
+      (requires True)
+      (ensures fun b ->
+         (b ==> (r.vput_key == fst store_kv /\
+                Some r.vput_value == snd store_kv /\
+                vput_app_success tsm r)))
+  = if r.vput_key = fst store_kv
+    then if Some r.vput_value = snd store_kv
+         then begin
+           VT.write_store t r.vput_slot (DValue (Some r.vput_value));
+           let b = true in
+           rewrite (VT.thread_state_inv_core t (vput_impl_tsm tsm r store_kv))
+                   (if b
+                    then VT.thread_state_inv_core t (vput_impl_tsm tsm r store_kv)
+                    else VT.thread_state_inv_core t tsm);
+           return b           
+         end
+         else begin
+           let b = false in
+           rewrite (VT.thread_state_inv_core t tsm)
+                   (if b
+                    then VT.thread_state_inv_core t (vput_impl_tsm tsm r store_kv)
+                    else VT.thread_state_inv_core t tsm);
+           return b
+         end
+    else begin
+      let b = false in
+      rewrite (VT.thread_state_inv_core t tsm)
+              (if b
+               then VT.thread_state_inv_core t (vput_impl_tsm tsm r store_kv)
+               else VT.thread_state_inv_core t tsm);
+      return b
+    end
+
+#push-options "--z3rlimit 50"
+let run_vput 
+  (#log_perm:perm)
+  (#log_bytes:Ghost.erased bytes)
+  (log_len: Ghost.erased U32.t)
+  (pl: runApp_payload)
+  (pl_pos:U32.t)
+  (log_array:larray U8.t log_len {
+    U32.v pl_pos + U32.v pl.rest.len <= Seq.length log_bytes /\
+    U32.v log_len == Seq.length log_bytes /\
+    Ghost.reveal pl.rest.ebytes == Seq.slice log_bytes (U32.v pl_pos) (U32.v pl_pos + U32.v pl.rest.len) })
+  (#out_bytes: Ghost.erased bytes)
+  (out_len:U32.t)
+  (out_offset:U32.t{U32.v out_offset <= Seq.length out_bytes})
+  (out:larray U8.t out_len)
+  (#tsm:M.thread_state_model)
+  (t:V.thread_state_t)
+  : ST verify_runapp_result
+       (V.thread_state_inv t tsm
+          `star`
+        A.pts_to log_array log_perm log_bytes
+          `star`
+        A.pts_to out full_perm out_bytes)
+       (fun res ->
+        A.pts_to log_array log_perm log_bytes
+          `star`
+        verify_runapp_entry_post tsm t pl out_bytes out_offset out res)
+       (requires not tsm.failed /\ pl.fid == S.vput_id)
+       (ensures fun _ -> True)
+  = let ropt = F.vput_args_parser log_len pl_pos pl.rest.len log_array in
+    match ropt with
+    | None -> return Run_app_parsing_failure
+    | Some (r, consumed) ->
+      if consumed = pl.rest.len
+      then begin
+        if U16.v r.vput_slot < U16.v AT.store_size
+        then begin
+          VT.elim_thread_state_inv t;
+          let kvopt = VT.read_store_app t r.vput_slot in
+          match kvopt with
+          | None ->
+            VT.intro_thread_state_inv t;
+            return Run_app_verify_failure
+          | Some (k, vopt) ->
+            let b = vput_impl t r (k, vopt) in
+            if b
+            then begin
+              rewrite (if b
+                       then VT.thread_state_inv_core t (vput_impl_tsm tsm r (k, vopt))
+                       else VT.thread_state_inv_core t tsm)
+                      (VT.thread_state_inv_core t (vput_impl_tsm tsm r (k, vopt)));
+              let tsm_write_slots =
+                TSM.write_slots tsm (vput_spec_slots r)
+                                    (vput_spec_out_vals tsm r) in
+              assert (Seq.equal (vput_impl_tsm tsm r (k, vopt)).store tsm_write_slots.store);
+              rewrite (VT.thread_state_inv_core t (vput_impl_tsm tsm r (k, vopt)))
+                      (VT.thread_state_inv_core t tsm_write_slots);
+
+              assume (Zeta.SeqAux.distinct_elems_comp (vput_spec_slots r));
+              assume (TSM.check_distinct_keys (Some?.v (TSM.read_slots tsm (vput_spec_slots r))));
+
+              let tsm_final =
+                {tsm_write_slots
+                 with app_results = Seq.snoc tsm_write_slots.app_results (vput_app_result tsm r);
+                      processed_entries=Seq.snoc tsm.processed_entries (RunApp pl)} in
+
+              assert (TSM.verify_step_model tsm (RunApp pl) == tsm_final);
+              assert (VT.tsm_entries_invariant tsm_final);
+
+              VT.restore_thread_state_inv_app t
+                (Seq.snoc tsm_write_slots.app_results (vput_app_result tsm r))
+                (Seq.snoc tsm.processed_entries (RunApp pl));
+
+              let wrote = 0ul in
+
+              intro_pure (n_out_bytes
+                            tsm
+                            (TSM.verify_step_model tsm (RunApp pl))
+                            out_offset
+                            wrote
+                            out_bytes
+                            out_bytes);
+              return (Run_app_success wrote)
+            end
+            else begin
+              rewrite (if b
+                       then VT.thread_state_inv_core t (vput_impl_tsm tsm r (k, vopt))
                        else VT.thread_state_inv_core t tsm)
                       (VT.thread_state_inv_core t tsm);
               VT.intro_thread_state_inv t;
@@ -215,80 +395,8 @@ let run_app_function #log_perm #log_bytes log_len pl pl_pos log_array
   #tsm t
   = if pl.fid = S.vget_id
     then run_vget log_len pl pl_pos log_array out_len out_offset out t
-    else admit__ ()
-
-    
-    // if pl.fid = KVS.vput_id
-    // then begin
-    //   assume (not tsm.failed);
-    //   let ropt = KVF.vput_args_parser log_len pl_pos pl.rest.len log_array in
-    //   match ropt with
-    //   | None -> return Run_app_parsing_failure
-    //   | Some (r, consumed) ->
-    //     //
-    //     // TODO: need to change the type in Zeta.Steel.Formats.fsti,
-    //     //       that file is generated by EverParse
-    //     //
-    //     assume (U16.v r.vput_slot < U16.v KAT.store_size);
-    //     let kvopt = VT.read_store t r.vput_slot in
-    //     match kvopt with
-    //     | None -> return Run_app_verify_failure
-    //     | Some kv ->
-    //       match kv.key, kv.value with
-    //       | InternalKey _, _ -> return Run_app_verify_failure
-    //       | _, MValue _ -> return Run_app_verify_failure
-    //       | ApplicationKey k, DValue v_store ->
-    //         if r.vput_key = k
-    //         then begin
-    //           VT.elim_thread_state_inv t;
-    //           VT.write_store #tsm t r.vput_slot (DValue (Some r.vput_value));
-    //           assert (ApplicationKey? (TSM.key_of_slot tsm r.vput_slot));
-    //           assert (TSM.has_slot tsm r.vput_slot);
-    //           assert (Map.contains aprm.tbl pl.fid);
-    //           assert (spec_app_parser pl.fid pl.rest.ebytes ==
-    //                   Some (((r.vput_key, r.vput_value), Seq.create 1 r.vput_slot), U32.v consumed));
-    //           assume (consumed == pl.rest.len);
-    //           assert (Zeta.SeqAux.distinct_elems_comp (Seq.create 1 r.vput_slot));
-    //           assert (
-    //             let slots = Seq.create 1 r.vput_slot in
-    //             let arg = r.vput_key, r.vput_value in
-    //             let recs = Some?.v (TSM.read_slots tsm (Seq.create 1 r.vput_slot)) in
-    //             let out_vals = Seq.create 1 (App.DValue r.vput_value) in
-    //             let tsm' = {tsm with app_results=Seq.Properties.snoc tsm.app_results (| pl.fid, arg, recs, () |)} in
-    //             let tsm' = TSM.write_slots tsm' slots out_vals in
-    //             let tsm' = {tsm' with processed_entries = Seq.snoc tsm.processed_entries (RunApp pl)} in
-    //             tsm' == TSM.verify_step_model tsm (RunApp pl) /\
-    //             tsm' == {(VT.update_tsm_slot_value tsm r.vput_slot (DValue (Some r.vput_value))) with
-    //                      TSM.app_results=Seq.Properties.snoc tsm.app_results (| pl.fid, arg, recs, () |);
-    //                      TSM.processed_entries = Seq.snoc tsm.processed_entries (RunApp pl)});
-    //           let tsm' = {(VT.update_tsm_slot_value tsm r.vput_slot (DValue (Some r.vput_value))) with
-    //                      TSM.app_results=Seq.Properties.snoc tsm.app_results (| pl.fid, (r.vput_key, r.vput_value), (Some?.v (TSM.read_slots tsm (Seq.create 1 r.vput_slot))), () |);
-    //                      TSM.processed_entries = Seq.snoc tsm.processed_entries (RunApp pl)} in
-    //           restore_thread_state_inv_core_put t
-    //             (VT.update_tsm_slot_value tsm r.vput_slot (DValue (Some r.vput_value)))
-    //             (Seq.Properties.snoc tsm.app_results (| pl.fid, (r.vput_key, r.vput_value), (Some?.v (TSM.read_slots tsm (Seq.create 1 r.vput_slot))), () |))
-    //             (Seq.snoc tsm.processed_entries (RunApp pl));
-    //           assert (VT.tsm_entries_invariant tsm');
-    //           VT.intro_thread_state_inv #_ #tsm' t;
-    //           let wrote = 0ul in
-    //           assume (n_out_bytes
-    //                     tsm
-    //                     (TSM.verify_step_model tsm (RunApp pl))
-    //                     out_offset
-    //                     wrote
-    //                     out_bytes
-    //                     out_bytes);
-    //           intro_pure (n_out_bytes
-    //                         tsm
-    //                         (TSM.verify_step_model tsm (RunApp pl))
-    //                         out_offset
-    //                         wrote
-    //                         out_bytes
-    //                         out_bytes);
-    //           return (Run_app_success wrote)
-    //         end
-    //         else return Run_app_verify_failure
-    // end
-    // else return Run_app_verify_failure
+    else if pl.fid = S.vput_id
+    then run_vput log_len pl pl_pos log_array out_len out_offset out t
+    else return Run_app_parsing_failure
 
 let key_type_to_base_key _ = admit__ ()
